add stdlib functions specs

src/Primitive/BooleanVSTSpecDecoder.v
@@ -1,15 +1,14 @@
-Require Import Core.Core  Core.StructNormalizer VstLib Lib BooleanExecSpec ErrorWithWriter.
+Require Import ASN1V.Core.Core Core.StructNormalizer VstLib Stdlib
+        BooleanExecSpec ErrorWithWriter BCTVSTSpec.
 Require Import VST.floyd.proofauto Psatz.
-Require Import VST.floyd.library.
-Require Export VST.floyd.Funspec_old_Notation.
-Require Import BCTVSTSpec Clight.BOOLEAN.
-Require Import StructNormalizer.
+Require Import Clight.BOOLEAN.
 
 Definition Vprog : varspecs. mk_varspecs prog. Defined.
 Instance CompSpecs : compspecs. make_compspecs prog. Defined.
 
 Instance Change1 : change_composite_env CompSpecs BCTVSTSpec.CompSpecs.
 Proof. make_cs_preserve CompSpecs BCTVSTSpec.CompSpecs. Defined.
+
 Instance Change2 : change_composite_env BCTVSTSpec.CompSpecs CompSpecs.
 Proof. make_cs_preserve BCTVSTSpec.CompSpecs CompSpecs. Defined.
 
@@ -17,177 +16,80 @@ Open Scope Z.
 
 Section Boolean_ber_decode.
 
-Notation _asn_dec_rval_s_struct := (Tstruct _asn_dec_rval_s noattr).
-
-Definition asn_dec_rval_rep sh v code cons :=  
- (field_at sh _asn_dec_rval_s_struct 
-           [StructField _code]
-           (Vint (Int.repr code)) v *
-  field_at sh _asn_dec_rval_s_struct 
-           [StructField _consumed] 
-           (Vint (Int.repr cons)) v)%logic. 
-
 Definition bool_ber_decode_spec : ident * funspec :=
   DECLARE _BOOLEAN_decode_ber
-    WITH (* Context pointer *)
-         sh_ctx : share, ctx_b : block, ctx_ofs : ptrofs, ctx : val,
-         (* Type Descriptor pointer *)
+    WITH sh_ctx : share, ctx_b : block, ctx_ofs : ptrofs, ctx : val,
          sh_td : share, td_b : block, td_ofs : ptrofs, td : TYPE_descriptor,
-         (* Value double pointer *)
-         sh_val: share, bool_value : val, (* pointer can be null *)
-         (* Buffer pointer *)
+         sh_val: share, bool_value : val, 
          sh_buf : share, buf_b : block, buf_ofs : ptrofs, buf : list byte,
-         (* pointer to the return struct dec_rval *)                        
          sh_res : share, res_b : block, res_ofs : ptrofs,
          size : Z, tag_mode : Z,
-         bv : val, res : val,
-         gv : globals
-    PRE  [
-         __res OF (tptr (Tstruct _asn_dec_rval_s noattr)),
-         _opt_codec_ctx OF (tptr (Tstruct _asn_codec_ctx_s noattr)),
-         _td OF (tptr (Tstruct _asn_TYPE_descriptor_s noattr)),
-         _bool_value OF (tptr (tptr tvoid)),
-         _buf_ptr OF (tptr tvoid),
-         _size OF tuint,
-         _tag_mode OF tint]
-    PROP ( readable_share sh_ctx; 
-           readable_share sh_td; 
-           readable_share sh_buf;
-           writable_share sh_res;
-            writable_share sh_val;
-           is_pointer_or_null bv
-            )
-    LOCAL ( temp _opt_codec_ctx ctx;
-            temp _td (Vptr td_b td_ofs);
-            temp _bool_value bool_value;
-            temp _buf_ptr (Vptr buf_b buf_ofs);
-            temp _size (Vint (Int.repr size));
-            temp _tag_mode (Vint (Int.repr tag_mode));
-            temp __res res)
-    SEP (data_at sh_ctx (tptr (Tstruct _asn_codec_ctx_s noattr))
+         bv : val, res : val
+    PRE  [ tptr asn_dec_rval_s,
+          tptr asn_codec_ctx_s,
+          tptr type_descriptor_s,
+          tptr (tptr tvoid), tptr tvoid, tuint, tint ] 
+    PROP (is_pointer_or_null bv)
+    PARAMS (res; ctx; Vptr td_b td_ofs; bool_value;
+            Vptr buf_b buf_ofs; Vint (Int.repr size);
+              Vint (Int.repr tag_mode))
+    GLOBALS()
+    SEP (valid_pointer bv;
+         data_at sh_ctx (tptr asn_codec_ctx_s)
                    (Vptr ctx_b ctx_ofs) ctx;
-         data_at sh_td (Tstruct _asn_TYPE_descriptor_s noattr)
+         data_at sh_td type_descriptor_s
                    (TYPE_descriptor_rep td) (Vptr td_b td_ofs);
          data_at sh_buf (tarray tschar (Zlength buf)) (map Vbyte buf) 
                    (Vptr buf_b buf_ofs);
-        data_at sh_val (tptr tvoid) bv bool_value;
-        data_at_ sh_res _asn_dec_rval_s_struct res)
+        data_at Share.Rsh (tptr tvoid) bv bool_value;
+        data_at_ Share.Rsh asn_dec_rval_s res)
     POST [tvoid]
       PROP()
       LOCAL ()
       SEP( (* Unchanged by the execution : *)
-           data_at sh_ctx (tptr (Tstruct _asn_codec_ctx_s noattr))
-                   (Vptr ctx_b ctx_ofs) ctx;
-           data_at sh_td (Tstruct _asn_TYPE_descriptor_s noattr) 
-                   (TYPE_descriptor_rep td) (Vptr td_b td_ofs);
+           valid_pointer bv;
+           data_at sh_ctx (tptr asn_codec_ctx_s) (Vptr ctx_b ctx_ofs) ctx;
+           data_at sh_td type_descriptor_s (TYPE_descriptor_rep td) 
+                   (Vptr td_b td_ofs);
            data_at sh_buf (tarray tschar (Zlength buf)) (map Vbyte buf) 
                    (Vptr buf_b buf_ofs);
            (* Changes according to the exec spec *)
-           let RC_FAIL := asn_dec_rval_rep sh_res (Vptr res_b res_ofs) 2 0 in
+           let RC_FAIL := data_at sh_res asn_dec_rval_s 
+                                  (construct_dec_rval 2 0) res in
            if Val.eq bool_value Vnullptr 
            then RC_FAIL
-           else let res := bool_decoder td buf in
-           match res with
-           | Some (r, c) => asn_dec_rval_rep sh_res (Vptr res_b res_ofs) 0 c * 
-                            data_at sh_val (tptr tuchar) (Vbyte (bool_to_byte r)) bool_value
-           | None => RC_FAIL *
-                     data_at sh_val (tptr tuchar)
-                             (default_val (tptr tuchar)) bool_value
-           end).
+           else match bool_decoder td buf with
+                | Some (r, c) => 
+                  data_at sh_res asn_dec_rval_s (construct_dec_rval 0 c) res *
+                  data_at sh_val (tptr tuchar) (Vbyte (bool_to_byte r)) bool_value
+                | None => RC_FAIL *
+                         data_at sh_val (tptr tuchar)
+                                 (default_val (tptr tuchar)) bool_value
+                end).
 
-(* SearchAbout mem_mgr.
-SearchAbout malloc_token. *)
-
-Definition calloc_spec :=
-   DECLARE _calloc
-   WITH m : Z, n : Z, ls : list byte (*, gv : globals *)
-   PRE [ 1%positive OF size_t, 2%positive OF size_t ]
-       PROP (0 <= m <= Ptrofs.max_unsigned ;
-             0 <= n <= Ptrofs.max_unsigned ;
-             0 <= m * n <= Ptrofs.max_unsigned;
-             Zlength ls = (m * n)%Z )
-       LOCAL (temp 1%positive (Vptrofs (Ptrofs.repr m)); 
-              temp 2%positive (Vptrofs (Ptrofs.repr n)) (*;
-              gvars gv *))
-       SEP ((* mem_mgr gv *))
-    POST [ tptr tvoid ] EX p : val, EX t : type,
-       PROP (Forall (fun x => x = Byte.zero) ls)
-       LOCAL (temp ret_temp p)
-       SEP ((* mem_mgr gv; *)
-         if eq_dec p nullval then emp
-         else (malloc_token Ews t p *
-               data_at Ews (tarray tschar m) (map Vbyte ls) p)).
-          
-Definition Gprog2 := ltac:(with_library prog [calloc_spec; 
+Definition Gprog := ltac:(with_library prog [(_calloc, calloc_spec); 
                                               ber_check_tags_spec; 
                                               bool_ber_decode_spec]).
 
-Theorem bool_der_encode : semax_body Vprog Gprog2 
+Theorem bool_der_encode : semax_body Vprog Gprog 
            (normalize_function f_BOOLEAN_decode_ber composites) bool_ber_decode_spec.
 Proof.
   start_function.
-  forward.
-  forward.
-  forward_if True.
-  entailer!.
-  try autorewrite with sublist in *|-.
-  eapply denote_tc_test_eq_split.
-  admit.
-  entailer!.
-  forward_call (1, 4, [Byte.zero; Byte.zero; Byte.zero; Byte.zero]).
-  cbn.
-  nia.
-  Intros p.
-  forward.
-  forward.
-  forward_if.
-  destruct (eq_dec (fst p) nullval) eqn : N.
-  entailer!.
-  admit.
-  entailer!.
   repeat forward.
-  entailer!.
-  admit.
-  forward.
-  entailer!.
-  hint.
-  autorewrite with sublist in *|-.
-  admit.
-  admit.
-  forward.
-  entailer!.
-  forward_loop (PROP (True)
-     LOCAL (temp _st bv; temp _t'11 bv; lvar __res__1 _asn_dec_rval_s_struct v__res__1;
-     lvar _tmp_error _asn_dec_rval_s_struct v_tmp_error; lvar _length tint v_length;
-     lvar _rval _asn_dec_rval_s_struct v_rval; temp __res res; temp _opt_codec_ctx ctx;
-     temp _td (Vptr td_b td_ofs); temp _bool_value bool_value;
-     temp _buf_ptr (Vptr buf_b buf_ofs); temp _size (Vint (Int.repr size));
-     temp _tag_mode (Vint (Int.repr tag_mode)))
-     SEP (data_at_ Tsh _asn_dec_rval_s_struct v__res__1;
-     data_at_ Tsh _asn_dec_rval_s_struct v_tmp_error; data_at_ Tsh tint v_length;
-     data_at_ Tsh _asn_dec_rval_s_struct v_rval;
-     data_at sh_ctx (tptr (Tstruct _asn_codec_ctx_s noattr)) (Vptr ctx_b ctx_ofs) ctx;
-     data_at sh_td (Tstruct _asn_TYPE_descriptor_s noattr) (TYPE_descriptor_rep td)
-       (Vptr td_b td_ofs);
-     data_at sh_buf (tarray tschar (Zlength buf)) (map Vbyte buf) (Vptr buf_b buf_ofs);
-     data_at sh_val (tptr tvoid) bv bool_value; data_at_ sh_res _asn_dec_rval_s_struct res)) break: (PROP (True)
-     LOCAL (temp _st bv; temp _t'11 bv; lvar __res__1 _asn_dec_rval_s_struct v__res__1;
-     lvar _tmp_error _asn_dec_rval_s_struct v_tmp_error; lvar _length tint v_length;
-     lvar _rval _asn_dec_rval_s_struct v_rval; temp __res res; temp _opt_codec_ctx ctx;
-     temp _td (Vptr td_b td_ofs); temp _bool_value bool_value;
-     temp _buf_ptr (Vptr buf_b buf_ofs); temp _size (Vint (Int.repr size));
-     temp _tag_mode (Vint (Int.repr tag_mode)))
-     SEP (data_at_ Tsh _asn_dec_rval_s_struct v__res__1;
-     data_at_ Tsh _asn_dec_rval_s_struct v_tmp_error; data_at_ Tsh tint v_length;
-     data_at_ Tsh _asn_dec_rval_s_struct v_rval;
-     data_at sh_ctx (tptr (Tstruct _asn_codec_ctx_s noattr)) (Vptr ctx_b ctx_ofs) ctx;
-     data_at sh_td (Tstruct _asn_TYPE_descriptor_s noattr) (TYPE_descriptor_rep td)
-       (Vptr td_b td_ofs);
-     data_at sh_buf (tarray tschar (Zlength buf)) (map Vbyte buf) (Vptr buf_b buf_ofs);
-     data_at sh_val (tptr tvoid) bv bool_value; data_at_ sh_res _asn_dec_rval_s_struct res)).
-  entailer!.
-  forward.
-  entailer!.
+  forward_if (is_pointer_or_null bv).
+  - forward_call (1, sizeof(tint)).
+    cbn; nia.
+    Intros p.
+    forward.
+    forward.
+    break_if.
+    break_let.
+    simpl in e; subst.
+    forward_if.
+    repeat forward.
+    (* entailer!.
+    break_if.
+    + entailer! *)
 Admitted.
 
 End Boolean_ber_decode.
