src/Core/Core.v
@@ -4,4 +4,4 @@ Export ListNotations.
 From compcert Require Export Coqlib Integers Floats AST Ctypes Cop Clight Clightdefs.
 From compcert Require Export Maps Values Events Memory.
 
-Require Import StructTact.StructTactics.
+Require Export StructTact.StructTactics.
