src/Lib/Stdlib.v
@@ -1,0 +1,42 @@
+Require Import Core.Core.
+Require Import VST.floyd.proofauto.
+Require Import VST.floyd.library.
+
+Definition calloc_spec {cs : compspecs} :=
+   WITH m : Z, n : Z
+   PRE [ size_t, size_t ]
+       PROP (0 <= m <= Ptrofs.max_unsigned ;
+             0 <= n <= Ptrofs.max_unsigned ;
+             0 <= m * n <= Ptrofs.max_unsigned)
+       PARAMS (Vptrofs (Ptrofs.repr m); 
+               Vptrofs (Ptrofs.repr n)) 
+       SEP ()
+    POST [ tptr tvoid ] EX p : val, EX t : type, EX ls : list byte, 
+       PROP (Zlength ls = (m * n)%Z;
+               Forall (fun x => x = Byte.zero) ls)
+       LOCAL (temp ret_temp p)
+       SEP (if eq_dec p nullval then emp
+            else malloc_token Ews t p * (* p is valid and malloc_compatible for t *)
+                  data_at Ews (tarray tschar m) (map Vbyte ls) p).
+
+Definition memcpy_spec {cs : compspecs} :=
+    WITH qsh : share, psh: share, p: val, q: val, n: Z, contents: list int
+   PRE [ tptr tvoid, tptr tvoid, tuint ]
+       PROP (readable_share qsh; writable_share psh; 0 <= n <= Int.max_unsigned)
+       PARAMS (p; q; Vint (Int.repr n))
+       SEP (data_at qsh (tarray tuchar n) (map Vint contents) q;
+              memory_block psh n p)
+    POST [ tptr tvoid ]
+       PROP() LOCAL(temp ret_temp p)
+       SEP(data_at qsh (tarray tuchar n) (map Vint contents) q;
+             data_at psh (tarray tuchar n) (map Vint contents) p).
+
+Definition memset_spec {cs : compspecs}:=
+   WITH sh : share, p: val, n: Z, c: int
+   PRE [ tptr tvoid, tint, tuint ]
+       PROP (writable_share sh; 0 <= n <= Int.max_unsigned)
+       PARAMS (p; Vint c; Vint (Int.repr n))
+       SEP (memory_block sh n p)
+    POST [ tptr tvoid ]
+       PROP() LOCAL(temp ret_temp p)
+       SEP(data_at sh (tarray tuchar n) (list_repeat (Z.to_nat n) (Vint c)) p).
